proof/amd64/extracted/Keccak1600_Jazz.ec
@@ -655,7 +655,7 @@ module M = {
     var at:int;
     aT8 <- aT;
     aT <- (8 * (aT %/ 8));
-    if ((aT8 <> 0)) {
+    if (((aT8 %% 8) <> 0)) {
       (buf, _LEN, _TRAILB, aT8, w) <@ __m_ilen_read_upto8_at (buf, _LEN,
       _TRAILB, aT, aT8);
       st.[(aT %/ 8)] <- (st.[(aT %/ 8)] `^` w);
@@ -2211,8 +2211,6 @@ module M = {
   }
   proc __addstate_m_avx2 (st:W256.t Array7.t, aT:int, buf:int, _LEN:int,
                           _TRAILB:int) : W256.t Array7.t * int * int = {
-    var t64_1:W64.t;
-    var t128_0:W128.t;
     var r0:W256.t;
     var r1:W256.t;
     var t64_2:W64.t;
@@ -2227,17 +2225,8 @@ module M = {
     var r6:W256.t;
     var r2:W256.t;
     if ((aT < 8)) {
-      if (((aT = 0) /\ (8 <= _LEN))) {
-        r0 <- (VPBROADCAST_4u64 (loadW64 Glob.mem buf));
-        buf <- (buf + 8);
-        _LEN <- (_LEN - 8);
-        aT <- 8;
-      } else {
-        (buf, _LEN, _TRAILB, aT, t64_1) <@ __m_ilen_read_upto8_at (buf, 
-        _LEN, _TRAILB, 0, aT);
-        t128_0 <- (zeroextu128 t64_1);
-        r0 <- (VPBROADCAST_4u64 (truncateu64 t128_0));
-      }
+      (buf, _LEN, _TRAILB, aT, r0) <@ __m_ilen_read_bcast_upto8_at (buf,
+      _LEN, _TRAILB, 0, aT);
       st.[0] <- (st.[0] `^` r0);
     } else {
       
@@ -2276,10 +2265,8 @@ module M = {
       } else {
         
       }
-      r2 <-
-      (W256.of_int
-      (((W128.to_uint t128_2) %% (2 ^ 128)) +
-      ((2 ^ 128) * (W128.to_uint t128_1))));
+      r2 <- (zeroextu256 t128_2);
+      r2 <- (VINSERTI128 r2 t128_1 (W8.of_int 1));
       st.[2] <- (st.[2] `^` r2);
     } else {
       
